Prove correctness for stubbed weakest preconditions with mutual induction.

deps/poulet4/examples/IntExampleWeakestPre.v
@@ -29,9 +29,19 @@ Definition pred_env_popped (p: pred) (env: environment tag_t) :=
     end
 .
 
-Fixpoint weakest_precondition_expression (expr: Expression tag_t) (post_env: @pred (environment tag_t)) (post_val: @pred (Value tag_t)) : @pred (environment tag_t) :=
+Fixpoint weakest_precondition_expression
+    (expr: Expression tag_t)
+    (post_env: @pred (environment tag_t))
+    (post_val: @pred (Value tag_t))
+    : @pred (environment tag_t)
+:=
     pred_false
-with weakest_precondition_expression_lvalue (expr: Expression tag_t) (post_env: @pred (environment tag_t)) (post_val: @pred ValueLvalue) : @pred (environment tag_t) :=
+with weakest_precondition_expression_lvalue
+    (expr: Expression tag_t)
+    (post_env: @pred (environment tag_t))
+    (post_val: @pred ValueLvalue)
+    : @pred (environment tag_t)
+:=
     pred_false
 .
 
@@ -41,7 +51,8 @@ Lemma weakest_precondition_expression_correct:
             exists env_post val_post,
                 post env_post /\
                 post_val val_post /\
-                eval_expression tag_t tag expr env_pre = (inl val_post, env_post)
+                eval_expression tag_t tag expr env_pre
+                    = (inl val_post, env_post)
 .
 Proof.
     intros.
@@ -65,95 +76,162 @@ Proof.
     contradiction.
 Qed.
 
-Fixpoint weakest_precondition (stmt: Statement tag_t) (post: @pred (environment tag_t)) : @pred (environment tag_t) :=
+Fixpoint weakest_precondition_statement
+    (stmt: Statement tag_t)
+    (post: @pred (environment tag_t))
+    : @pred (environment tag_t)
+:=
+    let '(MkStatement _ _ stmt _) := stmt in
+    weakest_precondition_statement_pre stmt post
+with weakest_precondition_statement_pre
+    (stmt: StatementPreT tag_t)
+    (post: @pred (environment tag_t))
+    : @pred (environment tag_t)
+:=
     match stmt with
-    | MkStatement _ _ stmt' _ =>
-      match stmt' with
-      | StatBlock _ block =>
-        let inter := weakest_precondition_block block (pred_env_popped post) in
-        pred_env_pushed inter
-      | StatAssignment _ lhs rhs =>
-        let inter :=
-            fun env_inter =>
-            forall rval lval env_post,
-                (inl tt, env_post) = update_lvalue tag_t tag lval rval env_inter /\
-                post env_post
-        in
-        let inter' := weakest_precondition_expression rhs inter pred_true in
-        weakest_precondition_expression_lvalue lhs inter' pred_true
-      (* | StatMethodCall callee type_args args =>
-        fun env_pre => *)
-      | StatEmpty _ => post
-      | _ => pred_false
-      end
+    | StatBlock _ block =>
+      let inter := weakest_precondition_block block (pred_env_popped post) in
+      pred_env_pushed inter
+    | StatAssignment _ lhs rhs =>
+      let inter :=
+          fun env_inter =>
+          forall rval lval,
+              exists env_post,
+                  (inl tt, env_post)
+                    = update_lvalue tag_t tag lval rval env_inter /\
+                  post env_post
+      in
+      let inter' := weakest_precondition_expression rhs inter pred_true in
+      weakest_precondition_expression_lvalue lhs inter' pred_true
+    (* | StatMethodCall callee type_args args =>
+      fun env_pre => *)
+    | StatEmpty _ => post
+    | _ => pred_false
     end
-with weakest_precondition_block (block: Block tag_t) (post: @pred (environment tag_t)) : @pred (environment tag_t) :=
+with weakest_precondition_block
+    (block: Block tag_t)
+    (post: @pred (environment tag_t))
+    : @pred (environment tag_t)
+:=
     match block with
     | BlockEmpty _ _ => post
     | BlockCons _ stmt block' =>
       let inter := weakest_precondition_block block' post in
-      weakest_precondition stmt inter
+      weakest_precondition_statement stmt inter
     end
 .
 
-Lemma weakest_precondition_block_correct:
-    forall env_pre block post,
+Definition weakest_precondition_block_correct
+    (block: Block tag_t)
+:=
+    forall env_pre post,
         weakest_precondition_block block post env_pre ->
             exists env_post,
                 post env_post /\
                 eval_block tag_t tag block env_pre = (inl tt, env_post)
 .
-Admitted.
 
-Lemma weakest_precondition_correct:
-    forall env_pre prog post,
-        weakest_precondition prog post env_pre ->
+Definition weakest_precondition_statement_pre_correct
+    (stmt: StatementPreT tag_t)
+:=
+    forall env_pre post,
+        weakest_precondition_statement_pre stmt post env_pre ->
             exists env_post,
                 post env_post /\
-                eval_statement tag_t tag prog env_pre = (inl tt, env_post)
+                eval_statement_pre tag_t tag stmt env_pre = (inl tt, env_post)
+.
+
+Definition weakest_precondition_statement_correct
+    (stmt: Statement tag_t)
+:=
+    forall env_pre post,
+        weakest_precondition_statement stmt post env_pre ->
+            exists env_post,
+                post env_post /\
+                eval_statement tag_t tag stmt env_pre = (inl tt, env_post)
+.
+
+Lemma weakest_precondition_correctness:
+    forall stmt, weakest_precondition_statement_correct stmt
 .
 Proof.
     intros.
-    destruct prog.
-    induction stmt; try (unfold pred_false in H; simpl in H; contradiction).
-    - unfold weakest_precondition in H.
-      apply weakest_precondition_expression_lvalue_correct in H.
-      destruct H as [env_inter [val_rhs [H [_ eval_lvalue_result]]]].
-      apply weakest_precondition_expression_correct in H.
-      destruct H as [env_post [val_lhs [update_lvalue_result [_ eval_expression_result]]]].
+    apply statement_mut with
+        (tags_t := tag_t)
+        (P0 := weakest_precondition_statement_pre_correct)
+        (P1 := weakest_precondition_block_correct);
+        unfold weakest_precondition_statement_pre_correct;
+        intros;
+        try (simpl in H; unfold pred_false in H; contradiction).
+    - unfold weakest_precondition_statement_correct.
+      intros.
+      simpl in H0.
+      specialize (H env_pre post H0).
+      destruct H as [env_post [env_post_fits eval_statement_result]].
       exists env_post.
-      specialize (update_lvalue_result val_lhs val_rhs env_post).
-      split.
-      * intuition.
-      * unfold eval_statement; simpl.
-        unfold state_bind.
-        rewrite eval_lvalue_result.
-        rewrite eval_expression_result.
-        easy.
-    - simpl weakest_precondition in H.
-      unfold pred_env_pushed in H.
-      apply weakest_precondition_block_correct in H.
-      destruct H as [env_post [env_post_fits eval_block_result]].
+      split; [exact env_post_fits|].
+      rewrite <- eval_statement_result.
+      reflexivity.
+    - unfold weakest_precondition_statement_pre in H.
+      apply weakest_precondition_expression_lvalue_correct in H.
+      destruct H as [env_inter' [lval [H [_ eval_lvalue_result]]]].
+      apply weakest_precondition_expression_correct in H.
+      destruct H as [env_inter [rval [env_inter_prop [_ eval_expression_result]]]].
+      specialize (env_inter_prop rval lval).
+      destruct env_inter_prop as [env_post [update_lvalue_result env_post_fits]].
+      exists env_post.
+      split; [exact env_post_fits|].
+      unfold eval_statement_pre; simpl.
+      unfold state_bind.
+      rewrite eval_lvalue_result.
+      rewrite eval_expression_result.
+      rewrite update_lvalue_result.
+      reflexivity.
+    - simpl in H0.
+      unfold pred_env_pushed in H0.
+      unfold weakest_precondition_block_correct in H.
+      specialize (H (push_scope tag_t env_pre) (pred_env_popped post) H0).
+      destruct H as [env_post' [env_post_fits eval_block_result]].
       unfold pred_env_popped in env_post_fits.
-      case_eq (pop_scope tag_t env_post); intros.
-      * rewrite H in env_post_fits.
-        exists e.
-        split; try easy.
-        replace (eval_statement tag_t tag (MkStatement tag_t tags (StatBlock tag_t block) typ))
-          with (map_env tag_t (push_scope tag_t);;
-                eval_block tag_t tag block;;
-                lift_env_fn tag_t (pop_scope tag_t));
-          [|reflexivity].
-        simpl.
-        unfold state_bind.
-        simpl.
-        rewrite eval_block_result.
-        unfold lift_env_fn.
-        rewrite H.
-        reflexivity.
-      * rewrite H in env_post_fits.
-        contradiction.
-    - exists env_pre.
-      simpl in H.
-      split; try easy.
+      case_eq (pop_scope tag_t env_post');
+        intros;
+        rewrite H in env_post_fits;
+        try contradiction.
+      exists e.
+      split; [exact env_post_fits|].
+      replace (eval_statement_pre tag_t tag (StatBlock tag_t block))
+         with (map_env tag_t (push_scope tag_t);;
+               eval_block tag_t tag block;;
+               lift_env_fn tag_t (pop_scope tag_t));
+         [|reflexivity]; simpl.
+      unfold state_bind; simpl.
+      rewrite eval_block_result.
+      unfold lift_env_fn.
+      rewrite H.
+      reflexivity.
+    - simpl in H.
+      exists env_pre.
+      split; [exact H|].
+      reflexivity.
+    - unfold weakest_precondition_block_correct; intros.
+      unfold weakest_precondition_block in H.
+      exists env_pre.
+      split; [exact H|].
+      reflexivity.
+    - unfold weakest_precondition_block_correct.
+      intros.
+      simpl in H1.
+      apply H in H1.
+      destruct H1 as [env_inter [H1 eval_statement_result]].
+      apply H0 in H1.
+      destruct H1 as [env_post [env_post_fits eval_block_result]].
+      exists env_post.
+      split; [exact env_post_fits|].
+      replace (eval_block tag_t tag (BlockCons tag_t statement rest))
+         with (eval_statement tag_t tag statement;;
+               eval_block tag_t tag rest);
+         [|reflexivity]; simpl.
+      unfold state_bind; simpl.
+      rewrite eval_statement_result.
+      exact eval_block_result.
 Qed.
